proofs/fstar/extraction/Libcrux.Kem.Kyber.Conversions.fst
@@ -2,12 +2,12 @@ module Libcrux.Kem.Kyber.Conversions
 #set-options "--fuel 0 --ifuel 1 --z3rlimit 15"
 open Core
 
-let into_padded_array (#len: usize) (slice: slice u8) : array u8 v_LEN =
+let into_padded_array (#v_LEN: usize) (slice: slice u8) : array u8 v_LEN =
   let _:Prims.unit =
     if true
     then
       let _:Prims.unit =
-        if ~.((Core.Slice.len_under_impl slice <: usize) <=. v_LEN <: bool)
+        if ~.((Core.Slice.impl__len slice <: usize) <=. v_LEN <: bool)
         then
           Rust_primitives.Hax.never_to_any (Core.Panicking.panic "assertion failed: slice.len() <= LEN"
 
@@ -19,14 +19,12 @@ let into_padded_array (#len: usize) (slice: slice u8) : array u8 v_LEN =
   let out:array u8 v_LEN = Rust_primitives.Hax.repeat 0uy v_LEN in
   let out:array u8 v_LEN =
     Rust_primitives.Hax.update_at out
-      ({
-          Core.Ops.Range.Range.f_start = 0sz;
-          Core.Ops.Range.Range.f_end = Core.Slice.len_under_impl slice <: usize
-        })
-      (Core.Slice.copy_from_slice_under_impl (Core.Ops.Index.IndexMut.index_mut out
+      ({ Core.Ops.Range.f_start = sz 0; Core.Ops.Range.f_end = Core.Slice.impl__len slice <: usize }
+      )
+      (Core.Slice.impl__copy_from_slice (Core.Ops.Index.IndexMut.index_mut out
               ({
-                  Core.Ops.Range.Range.f_start = 0sz;
-                  Core.Ops.Range.Range.f_end = Core.Slice.len_under_impl slice <: usize
+                  Core.Ops.Range.f_start = sz 0;
+                  Core.Ops.Range.f_end = Core.Slice.impl__len slice <: usize
                 })
             <:
             slice u8)
@@ -36,58 +34,44 @@ let into_padded_array (#len: usize) (slice: slice u8) : array u8 v_LEN =
   in
   out
 
-class t_UpdatingArray (v_Self: Type) = { push:self -> slice u8 -> self }
+class t_UpdatingArray (#v_Self: Type) = {
+  [@@@ FStar.Tactics.Typeclasses.no_method]_super_447510783:t_UpdatingArray v_Self;
+  f_push:v_Self -> slice u8 -> v_Self
+}
 
-type t_UpdatableArray = {
+type t_UpdatableArray (#v_LEN: usize) = {
   f_value:array u8 v_LEN;
   f_pointer:usize
 }
 
-let new_under_impl (#len: usize) (value: array u8 v_LEN) : t_UpdatableArray v_LEN =
-  {
-    Libcrux.Kem.Kyber.Conversions.UpdatableArray.f_value = value;
-    Libcrux.Kem.Kyber.Conversions.UpdatableArray.f_pointer = 0sz
-  }
+let impl__new (#v_LEN: usize) (value: array u8 v_LEN) : t_UpdatableArray v_LEN =
+  { f_value = value; f_pointer = sz 0 }
 
-let array_under_impl (#len: usize) (self: t_UpdatableArray v_LEN) : array u8 v_LEN =
-  self.Libcrux.Kem.Kyber.Conversions.UpdatableArray.f_value
+let impl__array (#v_LEN: usize) (self: t_UpdatableArray v_LEN) : array u8 v_LEN = self.f_value
 
-let impl (#len: usize) : t_UpdatingArray (t_UpdatableArray v_LEN) =
+let impl_1 (#v_LEN: usize) : t_UpdatingArray (t_UpdatableArray v_LEN) =
   {
-    push
+    f_impl_1__push
     =
-    fun (#len: usize) (self: t_UpdatableArray v_LEN) (other: slice u8) ->
+    fun (#v_LEN: usize) (self: t_UpdatableArray v_LEN) (other: slice u8) ->
       let self:t_UpdatableArray v_LEN =
         {
           self with
-          Libcrux.Kem.Kyber.Conversions.UpdatableArray.f_value
+          f_value
           =
-          Rust_primitives.Hax.update_at (Libcrux.Kem.Kyber.Conversions.UpdatableArray.f_value self
-              <:
-              t_UpdatableArray v_LEN)
+          Rust_primitives.Hax.update_at (f_value self <: t_UpdatableArray v_LEN)
             ({
-                Core.Ops.Range.Range.f_start
+                Core.Ops.Range.f_start = self.f_pointer;
+                Core.Ops.Range.f_end
                 =
-                self.Libcrux.Kem.Kyber.Conversions.UpdatableArray.f_pointer;
-                Core.Ops.Range.Range.f_end
-                =
-                self.Libcrux.Kem.Kyber.Conversions.UpdatableArray.f_pointer +.
-                (Core.Slice.len_under_impl other <: usize)
-                <:
-                usize
+                self.f_pointer +! (Core.Slice.impl__len other <: usize) <: usize
               })
-            (Core.Slice.copy_from_slice_under_impl (Core.Ops.Index.IndexMut.index_mut self
-                      .Libcrux.Kem.Kyber.Conversions.UpdatableArray.f_value
+            (Core.Slice.impl__copy_from_slice (Core.Ops.Index.IndexMut.index_mut self.f_value
                     ({
-                        Core.Ops.Range.Range.f_start
+                        Core.Ops.Range.f_start = self.f_pointer;
+                        Core.Ops.Range.f_end
                         =
-                        self.Libcrux.Kem.Kyber.Conversions.UpdatableArray.f_pointer;
-                        Core.Ops.Range.Range.f_end
-                        =
-                        self.Libcrux.Kem.Kyber.Conversions.UpdatableArray.f_pointer +.
-                        (Core.Slice.len_under_impl other <: usize)
-                        <:
-                        usize
+                        self.f_pointer +! (Core.Slice.impl__len other <: usize) <: usize
                       })
                   <:
                   slice u8)
@@ -97,16 +81,10 @@ let impl (#len: usize) : t_UpdatingArray (t_UpdatableArray v_LEN) =
         }
       in
       let self:t_UpdatableArray v_LEN =
-        {
-          self with
-          Libcrux.Kem.Kyber.Conversions.UpdatableArray.f_pointer
-          =
-          self.Libcrux.Kem.Kyber.Conversions.UpdatableArray.f_pointer +.
-          (Core.Slice.len_under_impl other <: usize)
-        }
+        { self with f_pointer = self.f_pointer +! (Core.Slice.impl__len other <: usize) }
       in
       self
   }
 
 let to_unsigned_representative (fe: i32) : u16 =
-  cast (fe +. ((fe <<. 15l <: i32) &. Libcrux.Kem.Kyber.Constants.v_FIELD_MODULUS <: i32))
+  cast (fe +! ((fe >>! 15l <: i32) &. Libcrux.Kem.Kyber.Constants.v_FIELD_MODULUS <: i32)) <: u16
