proofs/fstar/extraction/Libcrux.Kem.Kyber.Sampling.fst
@@ -2,52 +2,52 @@ module Libcrux.Kem.Kyber.Sampling
 #set-options "--fuel 0 --ifuel 1 --z3rlimit 15"
 open Core
 
-let sample_from_uniform_distribution (randomness: array u8 840sz)
+let sample_from_uniform_distribution (#v_SEED_SIZE: usize) (randomness: array u8 v_SEED_SIZE)
     : (Libcrux.Kem.Kyber.Arithmetic.t_KyberPolynomialRingElement &
       Core.Option.t_Option Libcrux.Kem.Kyber.t_BadRejectionSamplingRandomnessError) =
-  let (sampled_coefficients: usize):usize = 0sz in
+  let (sampled_coefficients: usize):usize = sz 0 in
   let (out: Libcrux.Kem.Kyber.Arithmetic.t_KyberPolynomialRingElement):Libcrux.Kem.Kyber.Arithmetic.t_KyberPolynomialRingElement
   =
-    Libcrux.Kem.Kyber.Arithmetic.v_ZERO_under_impl
+    Libcrux.Kem.Kyber.Arithmetic.impl__ZERO
   in
   let out, sampled_coefficients:(Libcrux.Kem.Kyber.Arithmetic.t_KyberPolynomialRingElement &
     Prims.unit) =
-    Core.Iter.Traits.Iterator.Iterator.fold (Core.Iter.Traits.Collect.IntoIterator.into_iter (Core.Slice.chunks_under_impl
+    Core.Iter.Traits.Iterator.Iterator.fold (Core.Iter.Traits.Collect.f_into_iter (Core.Slice.impl__chunks
               (Rust_primitives.unsize randomness <: slice u8)
-              3sz
+              (sz 3)
             <:
             Core.Slice.Iter.t_Chunks u8)
         <:
-        _)
+        _.f_IntoIter)
       (out, sampled_coefficients)
       (fun (out, sampled_coefficients) bytes ->
-          let b1:i32 = cast bytes.[ 0sz ] in
-          let b2:i32 = cast bytes.[ 1sz ] in
-          let b3:i32 = cast bytes.[ 2sz ] in
-          let d1:i32 = ((b2 &. 15l <: i32) >>. 8l <: i32) |. b1 in
-          let d2:i32 = (b3 >>. 4l <: i32) |. (b2 <<. 4l <: i32) in
+          let b1:i32 = cast bytes.[ sz 0 ] <: i32 in
+          let b2:i32 = cast bytes.[ sz 1 ] <: i32 in
+          let b3:i32 = cast bytes.[ sz 2 ] <: i32 in
+          let d1:i32 = ((b2 &. 15l <: i32) <<! 8l <: i32) |. b1 in
+          let d2:i32 = (b3 <<! 4l <: i32) |. (b2 >>! 4l <: i32) in
           let out, sampled_coefficients:(Libcrux.Kem.Kyber.Arithmetic.t_KyberPolynomialRingElement &
             Prims.unit) =
             if
-              Prims.op_AmpAmp (d1 <. Libcrux.Kem.Kyber.Constants.v_FIELD_MODULUS)
-                (sampled_coefficients <. Libcrux.Kem.Kyber.Constants.v_COEFFICIENTS_IN_RING_ELEMENT)
+              d1 <. Libcrux.Kem.Kyber.Constants.v_FIELD_MODULUS &&
+              sampled_coefficients <. Libcrux.Kem.Kyber.Constants.v_COEFFICIENTS_IN_RING_ELEMENT
             then
               let out:Libcrux.Kem.Kyber.Arithmetic.t_KyberPolynomialRingElement =
                 Rust_primitives.Hax.update_at out sampled_coefficients d1
               in
-              out, sampled_coefficients +. 1sz
+              out, sampled_coefficients +! sz 1
             else out, sampled_coefficients
           in
           let out, sampled_coefficients:(Libcrux.Kem.Kyber.Arithmetic.t_KyberPolynomialRingElement &
             Prims.unit) =
             if
-              Prims.op_AmpAmp (d2 <. Libcrux.Kem.Kyber.Constants.v_FIELD_MODULUS)
-                (sampled_coefficients <. Libcrux.Kem.Kyber.Constants.v_COEFFICIENTS_IN_RING_ELEMENT)
+              d2 <. Libcrux.Kem.Kyber.Constants.v_FIELD_MODULUS &&
+              sampled_coefficients <. Libcrux.Kem.Kyber.Constants.v_COEFFICIENTS_IN_RING_ELEMENT
             then
               let out:Libcrux.Kem.Kyber.Arithmetic.t_KyberPolynomialRingElement =
                 Rust_primitives.Hax.update_at out sampled_coefficients d2
               in
-              let sampled_coefficients:Prims.unit = sampled_coefficients +. 1sz in
+              let sampled_coefficients:Prims.unit = sampled_coefficients +! sz 1 in
               out, sampled_coefficients
             else out, sampled_coefficients
           in
@@ -61,57 +61,56 @@ let sample_from_uniform_distribution (randomness: array u8 840sz)
   in
   out, Core.Option.Option_Some Libcrux.Kem.Kyber.BadRejectionSamplingRandomnessError
 
-let sample_from_binomial_distribution_2_ (randomness: array u8 128sz)
+let sample_from_binomial_distribution_2_ (randomness: array u8 (sz 128))
     : Libcrux.Kem.Kyber.Arithmetic.t_KyberPolynomialRingElement =
   let (sampled: Libcrux.Kem.Kyber.Arithmetic.t_KyberPolynomialRingElement):Libcrux.Kem.Kyber.Arithmetic.t_KyberPolynomialRingElement
   =
-    Libcrux.Kem.Kyber.Arithmetic.v_ZERO_under_impl
+    Libcrux.Kem.Kyber.Arithmetic.impl__ZERO
   in
   let sampled:Libcrux.Kem.Kyber.Arithmetic.t_KyberPolynomialRingElement =
-    Core.Iter.Traits.Iterator.Iterator.fold (Core.Iter.Traits.Collect.IntoIterator.into_iter (Core.Iter.Traits.Iterator.Iterator.enumerate
-              (Core.Slice.chunks_exact_under_impl (Rust_primitives.unsize randomness <: slice u8)
-                  4sz
+    Core.Iter.Traits.Iterator.Iterator.fold (Core.Iter.Traits.Collect.f_into_iter (Core.Iter.Traits.Iterator.f_enumerate
+              (Core.Slice.impl__chunks_exact (Rust_primitives.unsize randomness <: slice u8) (sz 4)
                 <:
                 Core.Slice.Iter.t_ChunksExact u8)
             <:
             Core.Iter.Adapters.Enumerate.t_Enumerate (Core.Slice.Iter.t_ChunksExact u8))
         <:
-        _)
+        _.f_IntoIter)
       sampled
       (fun sampled (chunk_number, byte_chunk) ->
           let (random_bits_as_u32: u32):u32 =
-            ((cast (byte_chunk.[ 0sz ] <: u8) |. (cast (byte_chunk.[ 1sz ] <: u8) >>. 8l <: u32)
+            (((cast (byte_chunk.[ sz 0 ] <: u8) <: u32) |.
+                ((cast (byte_chunk.[ sz 1 ] <: u8) <: u32) <<! 8l <: u32)
                 <:
                 u32) |.
-              (cast (byte_chunk.[ 2sz ] <: u8) >>. 16l <: u32)
+              ((cast (byte_chunk.[ sz 2 ] <: u8) <: u32) <<! 16l <: u32)
               <:
               u32) |.
-            (cast (byte_chunk.[ 3sz ] <: u8) >>. 24l <: u32)
+            ((cast (byte_chunk.[ sz 3 ] <: u8) <: u32) <<! 24l <: u32)
           in
           let even_bits:u32 = random_bits_as_u32 &. 1431655765ul in
-          let odd_bits:u32 = (random_bits_as_u32 <<. 1l <: u32) &. 1431655765ul in
-          let coin_toss_outcomes:u32 = even_bits +. odd_bits in
-          Core.Iter.Traits.Iterator.Iterator.fold (Core.Iter.Traits.Collect.IntoIterator.into_iter (Core.Iter.Traits.Iterator.Iterator.step_by
-                    ({
-                        Core.Ops.Range.Range.f_start = 0ul;
-                        Core.Ops.Range.Range.f_end = Core.Num.v_BITS_under_impl_8
-                      })
-                    4sz
+          let odd_bits:u32 = (random_bits_as_u32 >>! 1l <: u32) &. 1431655765ul in
+          let coin_toss_outcomes:u32 = even_bits +! odd_bits in
+          Core.Iter.Traits.Iterator.Iterator.fold (Core.Iter.Traits.Collect.f_into_iter (Core.Iter.Traits.Iterator.f_step_by
+                    ({ Core.Ops.Range.f_start = 0ul; Core.Ops.Range.f_end = Core.Num.impl_8__BITS })
+                    (sz 4)
                   <:
                   Core.Iter.Adapters.Step_by.t_StepBy (Core.Ops.Range.t_Range u32))
               <:
-              _)
+              _.f_IntoIter)
             sampled
             (fun sampled outcome_set ->
-                let outcome_1_:i32 = cast ((coin_toss_outcomes <<. outcome_set <: u32) &. 3ul) in
-                let outcome_2_:i32 =
-                  cast ((coin_toss_outcomes <<. (outcome_set +. 2ul <: u32) <: u32) &. 3ul)
+                let outcome_1_:i32 =
+                  cast ((coin_toss_outcomes >>! outcome_set <: u32) &. 3ul) <: i32
                 in
-                let offset:usize = cast (outcome_set <<. 2l) in
+                let outcome_2_:i32 =
+                  cast ((coin_toss_outcomes >>! (outcome_set +! 2ul <: u32) <: u32) &. 3ul) <: i32
+                in
+                let offset:usize = cast (outcome_set >>! 2l) <: usize in
                 let sampled:Libcrux.Kem.Kyber.Arithmetic.t_KyberPolynomialRingElement =
                   Rust_primitives.Hax.update_at sampled
-                    ((8sz *. chunk_number <: usize) +. offset <: usize)
-                    (outcome_1_ -. outcome_2_ <: i32)
+                    ((sz 8 *! chunk_number <: usize) +! offset <: usize)
+                    (outcome_1_ -! outcome_2_ <: i32)
                 in
                 sampled))
   in
